Change constructor representation to follow C backend, add primitive add operation

benchmarks/js/run_wasm_external_pp.js
@@ -1,0 +1,98 @@
+import { print_i63, print_compare, print_bool, print_nat_sexp, print_nat_notation, print_list_sexp, print_list_notation, print_option, print_prod, print_positive_sexp, print_N_sexp, print_Z_sexp, print_compcert_byte_sexp } from './modules/pp.js';
+
+const pp_map = {
+    "demo1": (val, dataView) => print_list_sexp(val, dataView, print_bool),
+    "demo2": (val, dataView) => print_list_sexp(val, dataView, print_bool),
+    "list_sum": print_nat_sexp,
+    "vs_easy": print_bool,
+    "vs_hard": print_bool,
+    "binom": print_nat_sexp,
+    "color": (val, dataView) => print_prod(val, dataView, print_Z_sexp, print_Z_sexp),
+    "sha_fast": (val, dataView) => print_list_sexp(val, dataView, print_compcert_byte_sexp),
+    "ack_3_9": print_nat_sexp,
+    "even_10000": print_bool,
+    "bernstein_yang": print_Z_sexp,
+    "sm_gauss_nat": (val, dataView) => print_option(val, dataView, print_nat_sexp),
+    "sm_gauss_N": (val, dataView) => print_option(val, dataView, print_N_sexp),
+    "addition": print_nat_notation,
+    "addition_primitive": print_i63
+};
+
+import { readFileSync } from 'fs';
+
+var args = process.argv.slice(2);
+if (args.length != 2) {
+    console.log("Expected two args: 0: path to folder containing wasm file to run, 1: program.");
+    console.log("e.g.: $ node ./js/run_wasm_external_pp.js ./ vs_easy");
+    process.exit(1);
+}
+
+let path = args[0];
+
+if (path.charAt(path.length - 1) != "/") { path = path + "/" }
+
+const program = args[1];
+
+function write_int (value) {
+    process.stdout.write(value.toString())
+}
+
+function write_char (value) {
+    var chr = String.fromCharCode(value);
+    process.stdout.write(chr);
+}
+
+let importObject = {
+    env: {
+        write_char: write_char,
+        write_int: write_int,
+    }
+};
+
+(async () => {
+    const start_startup = Date.now();
+    const bytes = readFileSync(path + `CertiCoq.Benchmarks.tests.${program}.wasm`);
+
+    const obj = await WebAssembly.instantiate(
+        new Uint8Array (bytes), importObject
+    );
+    const stop_startup = Date.now();
+    const time_startup = stop_startup - start_startup;
+
+    try {
+	const start_main = Date.now();
+        obj.instance.exports.main_function();
+        const stop_main = Date.now();
+        const time_main = stop_main - start_main;
+
+	let bytes = obj.instance.exports.bytes_used.value;
+        let time_pp = undefined;
+
+        if (obj.instance.exports.result_out_of_mem.value == 1) {
+            console.log("Ran out of memory.");
+            console.log(`Benchmark ${path}: {{"time_startup": "${time_startup}", "time_main": "${time_main}", "program": "${program}"}} (in ms)`);
+            process.exit(1);
+        } else {
+	    const pp_fun = pp_map[program];
+	    if (pp_fun) {
+		const memory = obj.instance.exports.memory;
+		const dataView = new DataView(memory.buffer);
+		const res_value = obj.instance.exports.result.value;
+		process.stdout.write("====>");
+
+		const start_pp = Date.now();
+		pp_fun(res_value, dataView);
+		const stop_pp = Date.now();
+		time_pp = stop_pp - start_pp;
+		process.stdout.write("\n");
+	    }
+	    else {
+		console.log(`No pretty function defined for program ${program}`);
+	    }
+        }
+
+	console.log(`Benchmark ${path}: {{"time_startup": "${time_startup}", "time_main": "${time_main}", "time_pp": "${time_pp}", "program": "${program}"}} (in ms)`);
+    } catch (error) {
+	console.log(error);
+	process.exit(1);
+    }})();
