theories/CodegenWasm/LambdaANF_to_Wasm.v
@@ -29,25 +29,34 @@ Definition max_constr_alloc_size := (max_constr_args * 4 + 4)%Z. (* bytes, don't
 Definition assert (b : bool) (err : string) : error Datatypes.unit :=
   if b then Ret tt else Err err.
 
+Definition get_ctor_ord (cenv : ctor_env) (t : ctor_tag) : error N:=
+  match M.get t cenv with
+  | Some c => Ret (ctor_ordinal c)
+  | None => Err ("Constructor with tag " ++ (string_of_positive t) ++ " in constructor expression not found in constructor environment")%bs
+  end.
+
+
 (* enforces predicate expression_restricted in the proof file *)
-Fixpoint check_restrictions (e : exp) : error Datatypes.unit :=
+Fixpoint check_restrictions (cenv : ctor_env) (e : exp) : error Datatypes.unit :=
   match e with
   | Econstr _ t ys e' =>
-       _ <- assert (Z.of_nat (Pos.to_nat t) <? Wasm_int.Int32.half_modulus)%Z
-                       "constructor tag too large" ;;
-       _ <- assert (Z.of_nat (Datatypes.length ys) <=? max_constr_args)%Z
-                 "found constructor with too many args, check max_constr_args";;
-       check_restrictions e'
+      ord <- get_ctor_ord cenv t ;;
+      _ <- assert (Z.of_N ord <? Wasm_int.Int32.half_modulus)%Z "Constructor ordinal too large" ;;
+      _ <- assert (Z.of_nat (Datatypes.length ys) <=? max_constr_args)%Z
+             "found constructor with too many args, check max_constr_args";;
+      check_restrictions cenv e'
   | Ecase x ms =>
-      _ <- sequence (map (fun p =>
-                           _ <- assert (Z.of_nat (Pos.to_nat (fst p)) <? Wasm_int.Int32.half_modulus)%Z
-                                 "constructor tag too large" ;;
-                           check_restrictions (snd p)) ms);; Ret tt
-  | Eproj _ _ _ _ e' => check_restrictions e'
+      (* _ <- check_case_list_ordinals cenv ms;; *)
+      _ <- sequence (map (fun '(t, e') =>
+                            ord <- get_ctor_ord cenv t ;;
+                            _ <- assert (Z.of_N ord <? Wasm_int.Int32.half_modulus)%Z "Constructor ordinal too large" ;;
+                            check_restrictions cenv e') ms) ;;
+      Ret tt
+  | Eproj _ _ _ _ e' => check_restrictions cenv  e'
   | Eletapp _ _ _ ys e' =>
       _ <- assert (Z.of_nat (Datatypes.length ys) <=? max_function_args)%Z
                 "found function application with too many function params, check max_function_args";;
-      check_restrictions e'
+      check_restrictions cenv e'
   | Efun fds e' =>
       _ <- assert (Z.of_nat (numOf_fundefs fds) <? max_num_functions)%Z
                 "too many functions, check max_num_functions";;
@@ -58,15 +67,15 @@ Fixpoint check_restrictions (e : exp) : error Datatypes.unit :=
                   _ <- assert (Z.of_nat (length ys) <=? max_function_args)%Z
                        "found fundef with too many function args, check max_function_args";;
                   _ <- (iter fds');;
-                  check_restrictions e'
+                  check_restrictions cenv e'
               end) fds);;
-      check_restrictions e'
+      check_restrictions cenv e'
   | Eapp _ _ ys => assert (Z.of_nat (Datatypes.length ys) <=? max_function_args)%Z
                         "found function application with too many function params, check max_function_args"
-  | Eprim_val _ _ e' => check_restrictions e'
-  | Eprim _ _ _ e' => check_restrictions e'
+  | Eprim_val _ _ e' => check_restrictions cenv e'
+  | Eprim _ _ _ e' => check_restrictions cenv e'
   | Ehalt _ => Ret tt
-   end.
+  end.
 
 (* ***** FUNCTIONS and GLOBALS ****** *)
 
@@ -104,7 +113,6 @@ Definition constr_alloc_ptr  : immediate := 1. (* ptr to beginning of constr all
 Definition result_var        : immediate := 2. (* final result *)
 Definition result_out_of_mem : immediate := 3.
 
-
 (* ***** MAPPINGS ****** *)
 Definition localvar_env := M.tree nat. (* maps variables to their id (id=index in list of local vars) *)
 Definition fname_env    := M.tree nat. (* maps function variables to their id (id=index in list of functions) *)
@@ -131,11 +139,17 @@ Fixpoint arg_list (n : nat) : list (immediate * value_type) :=
 Definition nat_to_i32 (n : nat) :=
   Wasm_int.Int32.repr (BinInt.Z.of_nat n).
 
+Definition nat_to_i64 (n : nat) :=
+  Wasm_int.Int64.repr (BinInt.Z.of_nat n).
+
 Definition N_to_i32 (n : N) :=
   Wasm_int.Int32.repr (Z.of_N n).
 
 Definition nat_to_value (n : nat) :=
   VAL_int32 (nat_to_i32 n).
+
+Definition nat_to_value64 (n : nat) :=
+  VAL_int64 (nat_to_i64 n).
 
 Definition Z_to_value (z : Z) :=
   VAL_int32 (Wasm_int.Int32.repr z).
@@ -162,6 +176,7 @@ Definition instr_local_var_read (nenv : name_env) (lenv : localvar_env) (fenv : 
 
     else var <- translate_var nenv lenv v "instr_local_var_read: normal var";;
          Ret (BI_get_local var).
+
 
 
 (* ***** GENERATE PRETTY PRINTER FUNCTION FOR CONSTRUCTOR-S-EXPRESSIONS ****** *)
@@ -255,10 +270,10 @@ Definition generate_constr_pp_function (cenv : ctor_env) (nenv : name_env) (e : 
   blocks <- sequence (map (generate_constr_pp_single_constr cenv nenv) tags) ;;
 
   let body := (concat blocks) ++
-              (instr_write_string " <can't print constr: ") ++ (* e.g. could be fn-pointer or env-pointer *)
-              [ BI_get_local 0 (* param: ptr to constructor *)
-              ; BI_call write_int_function_idx
-              ] ++ instr_write_string ">" in
+                      ((instr_write_string " <can't print constr: ") ++ (* e.g. could be fn-pointer or env-pointer *)
+                          [ BI_get_local 0 (* param: ptr to constructor *)
+                            ; BI_call write_int_function_idx
+                          ] ++ instr_write_string ">" ) in
 
   let _ := ")"  (* hack to fix syntax highlighting bug *)
 
@@ -329,17 +344,9 @@ Definition translate_call (nenv : name_env) (lenv : localvar_env) (fenv : fname_
 
 (* **** TRANSLATE PRIMITIVE VALUES **** *)
 
-Definition to_int64 (i : PrimInt63.int) : Wasm_int.Int64.T.
-  exists (Uint63.to_Z i)%Z.
-  pose proof (Uint63.to_Z_bounded i).
-  unfold Uint63.wB in H. unfold Wasm_int.Int64.modulus, Wasm_int.Int64.wordsize, Integers.Wordsize_64.wordsize.
-  unfold Uint63.size in H. rewrite two_power_nat_correct. unfold Zpower_nat. simpl.
-  destruct H. split; lia.
-Defined.
-
-Definition translate_primitive (p : AstCommon.primitive) :=
+Definition translate_primitive_value (p : AstCommon.primitive) : error Wasm_int.Int64.int :=
   match projT1 p as tag return prim_value tag -> error Wasm_int.Int64.T with
-  | AstCommon.primInt => fun i => Ret (to_int64 i)
+  | AstCommon.primInt => fun i => Ret (Wasm_int.Int64.repr (Uint63.to_Z i))
   | AstCommon.primFloat => fun f => Err "TODO"
   end (projT2 p).
 
@@ -383,16 +390,15 @@ Fixpoint set_constructor_args (nenv : name_env) (lenv : localvar_env) (fenv : fn
 
 
 Definition store_constructor (nenv : name_env) (cenv : ctor_env) (lenv : localvar_env) (fenv : fname_env) (c : ctor_tag) (ys : list cps.var) : error (list basic_instruction) :=
-  let ctor_id := Pos.to_nat c in
+  ord <- get_ctor_ord cenv c ;;
   set_constr_args <- set_constructor_args nenv lenv fenv ys 0;;
   Ret ([ BI_get_global global_mem_ptr
        ; BI_set_global constr_alloc_ptr
 
        (* set tag *)
        ; BI_get_global constr_alloc_ptr
-       ; BI_const (nat_to_value ctor_id)
+       ; BI_const (nat_to_value (N.to_nat ord))
        ; BI_store T_i32 None 2%N 0%N (* 0: offset, 2: 4-byte aligned, alignment irrelevant for semantics *)
-
        (* increase gmp by 4 *)
        ; BI_get_global global_mem_ptr
        ; BI_const (nat_to_value 4)
@@ -401,39 +407,113 @@ Definition store_constructor (nenv : name_env) (cenv : ctor_env) (lenv : localva
 
        ] ++ set_constr_args).
 
-Fixpoint create_case_nested_if_chain (boxed : bool) (v : immediate) (es : list (ctor_tag * list basic_instruction)) : list basic_instruction :=
+(* **** TRANSLATE PRIMITIVE OPERATIONS **** *)
+
+Definition primInt63ModPath : Kernames.modpath :=
+  Kernames.MPfile ["Coq"%bs ; "Numbers"%bs ; "Cyclic"%bs ; "Int63"%bs ; "PrimInt63"%bs ].
+
+Definition primInt63Add : Kernames.kername := (primInt63ModPath, "add"%bs).
+
+Definition primInt63Sub : Kernames.kername := (primInt63ModPath, "sub"%bs).
+
+Definition primInt63Mul : Kernames.kername := (primInt63ModPath, "mul"%bs).
+
+Definition primInt63Div : Kernames.kername := (primInt63ModPath, "div"%bs).
+
+Definition primInt63Mod : Kernames.kername := (primInt63ModPath, "mod"%bs).
+
+Definition primInt63Land : Kernames.kername := (primInt63ModPath, "land"%bs).
+
+Definition primInt63Lor : Kernames.kername := (primInt63ModPath, "lor"%bs).
+
+Definition primInt63Lxor : Kernames.kername := (primInt63ModPath, "lxor"%bs).
+
+Definition primInt63Lsl : Kernames.kername := (primInt63ModPath, "lsl"%bs).
+
+Definition primInt63Lsr : Kernames.kername := (primInt63ModPath, "lsr"%bs).
+
+Definition apply_binop_and_store_i64 (op : basic_instruction) y1 y2 :=
+  [ BI_get_global global_mem_ptr (* Address to store the result of the operation *)
+  ; BI_get_local y1
+  ; BI_load T_i64 None 2%N 0%N
+  ; BI_get_local y2
+  ; BI_load T_i64 None 2%N 0%N
+  ; op
+  (* Ensure that value fits in 63 bits *)
+  ; BI_const (VAL_int64 (Wasm_int.Int64.repr Wasm_int.Int64.half_modulus))
+  ; BI_binop T_i64 (Binop_i (BOI_rem SX_U))
+  ; BI_store T_i64 None 2%N 0%N
+  ; BI_get_global global_mem_ptr (* value to be stored in the let binding ('return value') *)
+  (* Increment global memory pointer to next free memory segment  *)
+  ; BI_get_global global_mem_ptr
+  ; BI_const (nat_to_value 8)
+  ; BI_binop T_i32 (Binop_i BOI_add)
+  ; BI_set_global global_mem_ptr ].
+
+Definition translate_primitive_arith_op nenv lenv kname y1 y2 : error (list basic_instruction) :=
+    y1_var <- translate_var nenv lenv y1 "translate primitive integer arithmetic operation 1st argument" ;;
+    y2_var <- translate_var nenv lenv y2 "translate primitive integer arithmetic operation 2nd argument" ;;
+    if Kername.eqb kname primInt63Add then
+      Ret (apply_binop_and_store_i64 (BI_binop T_i64 (Binop_i BOI_add)) y1_var y2_var)
+          (* else if Kername.eqb kname primInt63Sub then *)
+          (*        Ret (apply_binop_and_store_i64 (BI_binop T_i64 (Binop_i BOI_sub)) y1_var y2_var) *)
+          (* else if Kername.eqb kname primInt63Mul then *)
+          (*        Ret (apply_binop_and_store_i64 (BI_binop T_i64 (Binop_i BOI_mul)) y1_var y2_var) *)
+          (* else if Kername.eqb kname primInt63Div then *)
+          (*        Ret (apply_binop_and_store_i64 (BI_binop T_i64 (Binop_i (BOI_div SX_U))) y1_var y2_var) *)
+          (* else if Kername.eqb kname primInt63Mod then *)
+          (*        Ret (apply_binop_and_store_i64 (BI_binop T_i64 (Binop_i (BOI_rem SX_U))) y1_var y2_var) *)
+          (* else if Kername.eqb kname primInt63Land then *)
+          (*        Ret (apply_binop_and_store_i64 (BI_binop T_i64 (Binop_i BOI_and)) y1_var y2_var) *)
+          (* else if Kername.eqb kname primInt63Lor then *)
+          (*        Ret (apply_binop_and_store_i64 (BI_binop T_i64 (Binop_i BOI_or)) y1_var y2_var) *)
+          (* else if Kername.eqb kname primInt63Lxor then *)
+          (*        Ret (apply_binop_and_store_i64 (BI_binop T_i64 (Binop_i BOI_xor)) y1_var y2_var) *)
+          (* else if Kername.eqb kname primInt63Lsl then *)
+          (*        Ret (apply_binop_and_store_i64 (BI_binop T_i64 (Binop_i BOI_shl)) y1_var y2_var) *)
+          (* else if Kername.eqb kname primInt63Lsr then *)
+          (*        Ret (apply_binop_and_store_i64 (BI_binop T_i64 (Binop_i (BOI_shr SX_U))) y1_var y2_var) *)
+    else
+      Err ("Unknown primitive arithmetic operator: " ++ (Kernames.string_of_kername kname))%bs.
+
+Definition translate_primitive_operation (nenv : name_env) (lenv : localvar_env) (x_var : immediate) (p : (kername * string * bool * nat)) (args : list var) : error (list basic_instruction) :=
+  let '(kname, _, _, _) := p in
+  match args with
+  | [ y1 ; y2 ] =>
+      op_instrs <- translate_primitive_arith_op nenv lenv kname y1 y2 ;;
+      Ret (op_instrs ++ [ BI_set_local x_var ])
+  | _ =>
+      Err "Only primitive operations with two arguments are supported"
+  end.
+
+Fixpoint create_case_nested_if_chain (boxed : bool) (v : immediate) (es : list (N * list basic_instruction)) : list basic_instruction :=
   match es with
   | [] => [ BI_unreachable ]
-  | (t, instrs) :: tl =>
+  | (ord, instrs) :: tl =>
       (* if boxed (pointer), then load tag from memory;
-         otherwise, obtain tag from unboxed representation ( tag = (repr >> 1) )
+         otherwise, the unboxed representation is (ord << 1) + 1 = 2 * ord + 1.
        *)
       BI_get_local v ::
         (if boxed then
-           [ BI_load T_i32 None 2%N 0%N ; BI_const (nat_to_value (Pos.to_nat t)) ]
+           [ BI_load T_i32 None 2%N 0%N ; BI_const (nat_to_value (N.to_nat ord)) ]
          else
-           [ BI_const (nat_to_value (Pos.to_nat (2 * t + 1))) ]) ++
+           [ BI_const (nat_to_value (N.to_nat (2 * ord + 1)%N)) ]) ++
         [ BI_relop T_i32 (Relop_i ROI_eq)
         ; BI_if (Tf nil nil) instrs (create_case_nested_if_chain boxed v tl) ]
   end.
 
-
 (* ***** TRANSLATE EXPRESSIONS (except fundefs) ****** *)
 
-Fixpoint translate_body (nenv : name_env) (cenv : ctor_env) (lenv: localvar_env) (fenv : fname_env) (e : exp) : error (list basic_instruction) :=
+Fixpoint translate_body (nenv : name_env) (cenv : ctor_env) (lenv: localvar_env) (fenv : fname_env) (penv : prim_env) (e : exp) : error (list basic_instruction) :=
    match e with
    | Efun fundefs e' => Err "unexpected nested function definition"
    | Econstr x tg ys e' =>
-      following_instr <- translate_body nenv cenv lenv fenv e' ;;
+      following_instr <- translate_body nenv cenv lenv fenv penv e' ;;
       x_var <- translate_var nenv lenv x "translate_body constr";;
       match ys with
-      | [] => Ret ([ BI_const (nat_to_value (Pos.to_nat tg)) (* Nullary constructor *)
-                  (* Unboxed representation ( (tag << 1) + 1 ) *)
-                  ; BI_const (nat_to_value 1)
-                  ; BI_binop T_i32 (Binop_i BOI_shl)
-                  ; BI_const (nat_to_value 1)
-                  ; BI_binop T_i32 (Binop_i BOI_add)
-                  ; BI_set_local x_var ] ++ following_instr)
+      | [] =>
+          ord <- get_ctor_ord cenv tg ;;
+          Ret ([ BI_const (nat_to_value (N.to_nat (2 * ord + 1)%N)) ; BI_set_local x_var ] ++ following_instr)
       | _ => (* n > 0 ary constructor  *)
           (* Boxed representation *)
           store_constr <- store_constructor nenv cenv lenv fenv tg ys;;
@@ -452,17 +532,18 @@ Fixpoint translate_body (nenv : name_env) (cenv : ctor_env) (lenv: localvar_env)
       end
    | Ecase x arms =>
       let fix translate_case_branch_expressions (arms : list (ctor_tag * exp))
-        : error (list (ctor_tag * list basic_instruction) * list (ctor_tag  * list basic_instruction)) :=
+        : error (list (N * list basic_instruction) * list (N  * list basic_instruction)) :=
         match arms with
         | [] => Ret ([], [])
         | (t, e)::tl =>
-            instrs <- translate_body nenv cenv lenv fenv e ;;
+            instrs <- translate_body nenv cenv lenv fenv penv e ;;
             '(arms_boxed, arms_unboxed) <- translate_case_branch_expressions tl ;;
+            ord <- get_ctor_ord cenv t ;;
             arity <- get_ctor_arity cenv t ;;
             if arity =? 0 then
-              Ret (arms_boxed, (t, instrs) :: arms_unboxed)
+              Ret (arms_boxed, (ord, instrs) :: arms_unboxed)
             else
-              Ret ((t, instrs) :: arms_boxed, arms_unboxed)
+              Ret ((ord, instrs) :: arms_boxed, arms_unboxed)
         end
       in
       x_var <- translate_var nenv lenv x "translate_body case" ;;
@@ -477,7 +558,7 @@ Fixpoint translate_body (nenv : name_env) (cenv : ctor_env) (lenv: localvar_env)
            ])
 
    | Eproj x tg n y e' =>
-      following_instr <- translate_body nenv cenv lenv fenv e' ;;
+      following_instr <- translate_body nenv cenv lenv fenv penv e' ;;
       y_var <- translate_var nenv lenv y "translate_body proj y";;
       x_var <- translate_var nenv lenv x "translate_body proj x";;
 
@@ -490,7 +571,7 @@ Fixpoint translate_body (nenv : name_env) (cenv : ctor_env) (lenv: localvar_env)
 
    | Eletapp x f ft ys e' =>
       x_var <- translate_var nenv lenv x "translate_body proj x";;
-      following_instr <- translate_body nenv cenv lenv fenv e' ;;
+      following_instr <- translate_body nenv cenv lenv fenv penv e' ;;
       instr_call <- translate_call nenv lenv fenv f ys false;;
 
       Ret (instr_call ++ [ BI_get_global result_out_of_mem
@@ -504,9 +585,9 @@ Fixpoint translate_body (nenv : name_env) (cenv : ctor_env) (lenv: localvar_env)
    | Eapp f ft ys => translate_call nenv lenv fenv f ys true
 
    | Eprim_val x p e' =>
-       following_instrs <- translate_body nenv cenv lenv fenv e' ;;
+       following_instrs <- translate_body nenv cenv lenv fenv penv e' ;;
        x_var <- translate_var nenv lenv x "translate_body prim val" ;;
-       val <- translate_primitive p ;;
+       val <- translate_primitive_value p ;;
        Ret ([ BI_const (N_to_value page_size)
             ; BI_call grow_mem_function_idx
             ; BI_get_global result_out_of_mem
@@ -526,8 +607,23 @@ Fixpoint translate_body (nenv : name_env) (cenv : ctor_env) (lenv: localvar_env)
             ; BI_set_global global_mem_ptr
             ] ++ following_instrs)
 
-   | Eprim x p ys e' => Err "translating prim to Wasm not supported yet"
-
+   | Eprim x p ys e' => (* Err "temp" *)
+       match M.get p penv with
+       | None => Err "Primitive operation not found in prim_env"
+       | Some p' =>
+           following_instrs <- translate_body nenv cenv lenv fenv penv e';;
+           x_var <- translate_var nenv lenv x "translate_exp prim op" ;;
+           instrs <- translate_primitive_operation nenv lenv x_var p' ys ;;
+           Ret ( [ BI_const (N_to_value page_size)
+                 ; BI_call grow_mem_function_idx
+                 ; BI_get_global result_out_of_mem
+                 ; BI_const (nat_to_value 1)
+                 ; BI_relop T_i32 (Relop_i ROI_eq)
+                 ; BI_if (Tf [] [])
+                     [ BI_return ]
+                     []
+                 ] ++ instrs ++ following_instrs)
+       end
    | Ehalt x =>
      x_var <- translate_var nenv lenv x "translate_body halt";;
      Ret [ BI_get_local x_var; BI_set_global result_var; BI_return ]
@@ -569,13 +665,13 @@ Definition function_export_name (nenv : name_env) (v : cps.var) : string :=
                               end)
                     bytes).
 
-Definition translate_function (nenv : name_env) (cenv : ctor_env) (fenv : fname_env)
+Definition translate_function (nenv : name_env) (cenv : ctor_env) (fenv : fname_env) (penv : prim_env)
                               (f : cps.var) (args : list cps.var) (body : exp) : error wasm_function :=
   let locals := collect_local_variables body in
   let lenv := create_local_variable_mapping (args ++ locals) in
 
   fn_idx <- translate_var nenv fenv f "translate function" ;;
-  body_res <- translate_body nenv cenv lenv fenv body ;;
+  body_res <- translate_body nenv cenv lenv fenv penv body ;;
   Ret {| fidx := fn_idx
        ; export_name := function_export_name nenv f
        ; type := Tf (map (fun _ => T_i32) args) []
@@ -583,15 +679,17 @@ Definition translate_function (nenv : name_env) (cenv : ctor_env) (fenv : fname_
        ; body := body_res
        |}.
 
-Fixpoint translate_functions (nenv : name_env) (cenv : ctor_env) (fenv : fname_env)
+Fixpoint translate_functions (nenv : name_env) (cenv : ctor_env) (fenv : fname_env) (penv : prim_env)
                              (fds : fundefs) : error (list wasm_function) :=
   match fds with
   | Fnil => Ret []
   | Fcons x tg xs e fds' =>
-      fn <- translate_function nenv cenv fenv x xs e ;;
-      following <- translate_functions nenv cenv fenv fds' ;;
+      fn <- translate_function nenv cenv fenv penv x xs e ;;
+      following <- translate_functions nenv cenv fenv penv fds' ;;
       Ret (fn :: following)
   end.
+
+
 
 
 (* ***** MAIN: GENERATE COMPLETE WASM_MODULE FROM lambdaANF EXP ****** *)
@@ -602,7 +700,7 @@ Definition collect_function_vars (e : cps.exp) : list cps.var :=
       (fix iter (fds : fundefs) : list cps.var :=
           match fds with
           | Fnil => []
-          | Fcons x _ _ _ fds' => x :: (iter fds')
+          | Fcons x _ _ e' fds' => x :: (iter fds')
           end) fds
     | _ => []
     end.
@@ -628,9 +726,8 @@ Fixpoint table_element_mapping (len : nat) (startidx : nat) : list module_elemen
                |} :: (table_element_mapping len' (S startidx))
   end.
 
-
-Definition LambdaANF_to_Wasm (nenv : name_env) (cenv : ctor_env) (e : exp) : error (module * fname_env * localvar_env) :=
-  _ <- check_restrictions e;;
+Definition LambdaANF_to_Wasm (nenv : name_env) (cenv : ctor_env) (penv : prim_env) (e : exp) : error (module * fname_env * localvar_env) :=
+  _ <- check_restrictions cenv e;;
 
   let fname_mapping := create_fname_mapping e in
 
@@ -644,7 +741,7 @@ Definition LambdaANF_to_Wasm (nenv : name_env) (cenv : ctor_env) (e : exp) : err
                  end in
 
   fns <- match top_exp with
-         | Efun fds exp => translate_functions nenv cenv fname_mapping fds
+         | Efun fds exp => translate_functions nenv cenv fname_mapping penv fds
          | _ => Err "unreachable"
          end ;;
 
@@ -654,7 +751,7 @@ Definition LambdaANF_to_Wasm (nenv : name_env) (cenv : ctor_env) (e : exp) : err
                end;;
   let main_vars := collect_local_variables main_expr in
   let main_lenv := create_local_variable_mapping main_vars in
-  main_instr <- translate_body nenv cenv main_lenv fname_mapping main_expr ;;
+  main_instr <- translate_body nenv cenv main_lenv fname_mapping penv main_expr ;;
 
   let main_function := {| fidx := main_function_idx
                         ; export_name := main_function_name
@@ -664,6 +761,7 @@ Definition LambdaANF_to_Wasm (nenv : name_env) (cenv : ctor_env) (e : exp) : err
                         |}
   in
   let functions := [constr_pp_function; grow_mem_function; main_function] ++ fns in
+
   let exports := map (fun f => {| modexp_name := String.print f.(export_name)
                                 ; modexp_desc := MED_func (Mk_funcidx f.(fidx))
                                 |}) functions (* function exports for debug names *)
@@ -677,7 +775,7 @@ Definition LambdaANF_to_Wasm (nenv : name_env) (cenv : ctor_env) (e : exp) : err
                      ; modexp_desc := MED_global (Mk_globalidx result_var)
                     |} ::
                     {| modexp_name := String.print "memory"
-                    ; modexp_desc := MED_mem (Mk_memidx 0)
+                     ; modexp_desc := MED_mem (Mk_memidx 0)
                     |} :: nil
   in
 
@@ -686,12 +784,13 @@ Definition LambdaANF_to_Wasm (nenv : name_env) (cenv : ctor_env) (e : exp) : err
   let functions_final := map (fun f => {| modfunc_type := Mk_typeidx (match f.(type) with Tf args _ => length args end)
                                         ; modfunc_locals := f.(locals)
                                         ; modfunc_body := f.(body)
-                                        |}) functions in
+                                       |}) functions in
   let module :=
-      {| mod_types := list_function_types (Z.to_nat max_function_args) (* more than required, doesn't hurt*)
+      {| mod_types := (list_function_types (Z.to_nat max_function_args)) (* more than required, doesn't hurt*)
 
        ; mod_funcs := functions_final
        ; mod_tables := [ {| modtab_type := {| tt_limits := {| lim_min := N.of_nat (List.length fns + num_custom_funs)
+
                                                             ; lim_max := None |}
                                             ; tt_elem_type := ELT_funcref
                                             |} |}]
@@ -725,7 +824,6 @@ Definition LambdaANF_to_Wasm (nenv : name_env) (cenv : ctor_env) (e : exp) : err
                          ; imp_name := String.print write_int_function_name
                          ; imp_desc := ID_func 1
                          |} :: nil
-
        ; mod_exports := exports
        |}
        in
